theories/operations.v
@@ -10,9 +10,27 @@ Set Implicit Arguments.
 Unset Strict Implicit.
 Unset Printing Implicit Defensive.
 
-(* Placeholder for better array lookup in the future *)
+(* Placeholder for better array lookup in the future. *)
 Definition lookup_N {T: Type} (l: list T) (n: N) : option T :=
   List.nth_error l (N.to_nat n).
+
+(* A safe version that avoids stack overflowing when n is large, but slower. *)
+Definition lookup_N_safe {T: Type} (l: list T) (n: N) : option T :=
+  if (n <? N.of_nat (List.length l))%N then
+    List.nth_error l (N.to_nat n)
+  else None.
+
+Lemma lookup_N_safe_spec: forall {T: Type} (l: list T) (n:N),
+    lookup_N_safe l n = lookup_N l n.
+Proof.
+  move => T l n.
+  unfold lookup_N_safe.
+  destruct (n <? N.of_nat (length l))%N eqn:Hlt => //.
+  move/N.ltb_spec0 in Hlt.
+  symmetry.
+  apply List.nth_error_None.
+  by lias.
+Qed.
 
 Definition empty_t_context := Build_t_context nil nil nil nil nil nil nil nil nil None nil.
 
