Makefile
@@ -1,3 +1,8 @@
 default:
 	opam install .
 
+run_wast_local:
+	for wastfile in ./tests/wast/*.wast; do \
+		echo "Running: $$wastfile"; \
+		dune exec -- wasm_coq_interpreter --wast "$$wastfile"; \
+	done
